coq/Coqlib.v
@@ -16,3 +16,12 @@ Export ListNotations.
 From ExtLib Require Export
   Data.Monads.OptionMonad
   Structures.Monads.
+
+From Coq Require Export
+     ssreflect
+     ssrfun
+     ssrbool.
+
+Set Implicit Arguments.
+Unset Strict Implicit.
+Unset Printing Implicit Defensive.
